@prefix cc:      <http://creativecommons.org/ns#> .
@prefix dc:      <http://purl.org/dc/elements/1.1/>.
@prefix dcat:    <http://www.w3.org/ns/dcat#>.
@prefix dcterms: <http://purl.org/dc/terms/>.
@prefix disco:   <http://rdf-vocabulary.ddialliance.org/discovery#>.
@prefix owl:     <http://www.w3.org/2002/07/owl#>.
@prefix phdd:    <http://rdf-vocabulary.ddialliance.org/phdd#>.
@prefix rdf:     <http://www.w3.org/1999/02/22-rdf-syntax-ns#>.
@prefix rdfs:    <http://www.w3.org/2000/01/rdf-schema#>.
@prefix skos:    <http://www.w3.org/2004/02/skos/core#>.
@prefix xsd:     <http://www.w3.org/2001/XMLSchema#>.

#################################################################
# Ontology
#################################################################

<http://rdf-vocabulary.ddialliance.org/phdd> a owl:Ontology;
    dc:title
        "Physical Data Description (PHDD)"@en;
    rdfs:comment "Physical data description (PHDD) of existing or published data (tables) in a rectangular format. The data could be either represented in records with character-separated values (CSV) or in records with fixed length. PHDD could be used standalone or together with related vocabularies like Data Catalog Vocabulary (DCAT) or DDI-RDF Discovery.Descriptions in PHDD could be added to Web pages which provide tables in rectangular format. This would enable processing by programs of this data. The combined usage of PHDD, DDI-RDF Discovery, and DCAT would enable the creation of data repositories which provide metadata for the description of collections, for data discovery, and for processing of the data.PHDD is based on the DDI (Data Documentation Initiative, ddialliance.org) specification. This ontology is available at http://rdf-vocabulary.ddialliance.org/phdd, and uses the namespace prefix phdd."^^xsd:string ;
	dc:description <https://raw.githubusercontent.com/linked-statistics/physical-data-description/master/UML/phdd_web.png> ;
	dc:rights "This work is distributed under a Creative Commons Attribution License (http://creativecommons.org/licenses/by-nc-sa/3.0/us/)."@en ;
    dc:creator
"Joachim Wackerow","Thomas Bosch",
"Larry Hoyle";
    dc:contributor"Richard Cyganiak";
	dc:date "2014-05-25"^^xsd:string ;
    owl:versionInfo "0.1";
	cc:license <http://creativecommons.org/licenses/by-nc-sa/3.0/us/> .

#################################################################
# Classes
#################################################################

# Table
phdd:Table a rdfs:Class, owl:Class;
    rdfs:label "Table"@en;
	rdfs:comment "A table, which could be a rectangular file with character-separated values (CSV) or a rectangular file with fixed record length.This can be a subclass of 'Distribution' in Data Catalog Vocabulary (DCAT), see: http://www.w3.org/TR/vocab-dcat/#class-distribution.The equivalent class in DDI-RDF Discovery (Disco) is 'DataFile', see: http://rdf-vocabulary.ddialliance.org/discovery.html#datafile.Related element in DDI 3.2: p:PhysicalDataProductDDI 3.2 Documentation:  http://www.ddialliance.org/Specification/DDI-Lifecycle/3.2/XMLSchema/FieldLevelDocumentation/schemas/physicaldataproduct_xsd/elements/PhysicalDataProduct.html"@en;
    rdfs:subClassOf dcat:Distribution;owl:equivalentClass disco:DataFile;rdfs:subClassOf[ a owl:Restriction;  owl:onProperty phdd:isDescribedBy;  owl:onClass phdd:TableDescription;  owl:minCardinality 1;  owl:maxCardinality 1];rdfs:isDefinedBy <http://rdf-vocabulary.ddialliance.org/phdd>;rdfs:seeAlso <http://www.ddialliance.org/Specification/DDI-Lifecycle/3.2/XMLSchema/FieldLevelDocumentation/schemas/physicaldataproduct_xsd/elements/PhysicalDataProduct.html>.

#################################################################

# InputProgram
phdd:InputProgram a rdfs:Class, owl:Class;
    rdfs:label "Input Program"@en;rdfs:comment "Program or program statements for reading the data.Related element in DDI 3.2: r:CommandFileDDI 3.2 Documentation: http://www.ddialliance.org/Specification/DDI-Lifecycle/3.2/XMLSchema/FieldLevelDocumentation/schemas/reusable_xsd/elements/CommandFile.html"@en;
rdfs:subClassOf[ a owl:Restriction;  owl:onProperty [owl:inverseOf phdd:inputProgram];  owl:onClass phdd:TableDescription;  owl:maxCardinality 1];
    rdfs:isDefinedBy <http://rdf-vocabulary.ddialliance.org/phdd>;
    rdfs:seeAlso <http://www.ddialliance.org/Specification/DDI-Lifecycle/3.2/XMLSchema/FieldLevelDocumentation/schemas/reusable_xsd/elements/CommandFile.html>.

#################################################################
# TableDescription
phdd:TableDescription a rdfs:Class, owl:Class;
    rdfs:label "Table Description"@en;rdfs:comment "Description of a table by significant parameters."@en;
    rdfs:isDefinedBy <http://rdf-vocabulary.ddialliance.org/phdd>.

#################################################################
# TableStructure
phdd:TableStructure a rdfs:Class, owl:Class;
    rdfs:label "Table Structure"@en;rdfs:comment "The table properties described by default parameters of the data values."@en;
    rdfs:isDefinedBy <http://rdf-vocabulary.ddialliance.org/phdd>.

#################################################################
# FixedRecordLength
phdd:FixedRecordLength a rdfs:Class, owl:Class;
    rdfs:label "Fixed record length"@en;
	rdfs:comment "Detailed description of a table with fixed record length additionally to the common properties in 'TableStructure'."@en;
    rdfs:isDefinedBy <http://rdf-vocabulary.ddialliance.org/phdd>;rdfs:subClassOf phdd:TableStructure.

#################################################################
# Delimited
phdd:Delimited a rdfs:Class, owl:Class;
    rdfs:label "Delimited"@en;rdfs:comment "Detailed description of a table with character-separated values additionally to the common properties in 'TableStructure'."@en;
    rdfs:isDefinedBy <http://rdf-vocabulary.ddialliance.org/phdd>;rdfs:subClassOf phdd:TableStructure.

#################################################################
# Column
phdd:Column a rdfs:Class, owl:Class;
    rdfs:label "Column"@en;rdfs:comment "A column of a table. Other terms are variable or data item.Equivalent class in Disco: VariableDisco documentation: http://rdf-vocabulary.ddialliance.org/discovery.html#variable-and-variable-definitionEquivalent element in DDI 3.2: l:VariableDDI 3.2 Documentation:  http://www.ddialliance.org/Specification/DDI-Lifecycle/3.2/XMLSchema/FieldLevelDocumentation/schemas/logicalproduct_xsd/elements/Variable.html"@en;
    rdfs:isDefinedBy <http://rdf-vocabulary.ddialliance.org/phdd>;
    rdfs:isDefinedBy <http://www.ddialliance.org/Specification/DDI-Lifecycle/3.2/XMLSchema/FieldLevelDocumentation/schemas/logicalproduct_xsd/elements/Variable.html>;owl:equivalentClass disco:Variable.

#################################################################
# ColumnDescription
phdd:ColumnDescription a rdfs:Class, owl:Class;
    rdfs:label "Column description"@en;rdfs:comment "Detailed description of a column. It comprehends common properties of delimited column and fixed column data."@en;
    rdfs:isDefinedBy <http://rdf-vocabulary.ddialliance.org/phdd>.

#################################################################
# DelimitedColumnDescription
phdd:DelimitedColumnDescription a rdfs:Class, owl:Class;
    rdfs:label "Delimited column description"@en;rdfs:comment "Detailed description of a column in CSV data additionally to the common properties in 'ColumnDescription'."@en;
    rdfs:isDefinedBy <http://rdf-vocabulary.ddialliance.org/phdd>;rdfs:subClassOf phdd:ColumnDescription.

#################################################################
# FixedColumnDescription
phdd:FixedColumnDescription a rdfs:Class, owl:Class;
    rdfs:label "fixed column description"@en;rdfs:comment "Detailed description of a column in fixed record length data in addition to the common properties in 'ColumnDescription'."@en;
    rdfs:isDefinedBy <http://rdf-vocabulary.ddialliance.org/phdd>;rdfs:subClassOf phdd:ColumnDescription.

#################################################################
# Datatype properties
#################################################################

# programFileName
phdd:programFileName a rdf:Property, owl:DatatypeProperty;
    rdfs:label "Program file name"@en;rdfs:comment "File name or URI of the input program."@en;
    rdfs:domain phdd:InputProgram;
    rdfs:range xsd:string;
    rdfs:isDefinedBy <http://rdf-vocabulary.ddialliance.org/phdd>.

# softwareType
phdd:softwareType a rdf:Property, owl:DatatypeProperty;
    rdfs:label "Software type"@en;rdfs:comment "Software or program language used of the program for reading the data.Equivalent element in DDI 3.2: r:ProgramLanguageDDI 3.2 Documentation: http://www.ddialliance.org/Specification/DDI-Lifecycle/3.2/XMLSchema/FieldLevelDocumentation/schemas/reusable_xsd/elements/ProgramLanguage.html"@en;
    rdfs:domain phdd:InputProgram;
    rdfs:range xsd:string;
    rdfs:isDefinedBy <http://rdf-vocabulary.ddialliance.org/phdd>.
# programVersion
phdd:programVersion a rdf:Property, owl:DatatypeProperty;
    rdfs:label "Program version"@en;rdfs:comment "Version of the software used of the program for reading the data."@en;
    rdfs:domain phdd:InputProgram;
    rdfs:range xsd:string;
    rdfs:isDefinedBy <http://rdf-vocabulary.ddialliance.org/phdd>.
# caseQuantity
phdd:caseQuantity a rdf:Property, owl:DatatypeProperty;
    rdfs:label "Case quantity"@en;rdfs:comment "Number of cases or observations in the table.Equivalent element in DDI 3.2: pi:CaseQuantityDDI 3.2 Documentation: http://www.ddialliance.org/Specification/DDI-Lifecycle/3.2/XMLSchema/FieldLevelDocumentation/schemas/physicalinstance_xsd/elements/CaseQuantity.html"@en;
    rdfs:domain phdd:TableDescription;
    rdfs:range xsd:nonNegativeInteger;
    rdfs:isDefinedBy <http://rdf-vocabulary.ddialliance.org/phdd>;
    rdfs:isDefinedBy <http://www.ddialliance.org/Specification/DDI-Lifecycle/3.2/XMLSchema/FieldLevelDocumentation/schemas/physicalinstance_xsd/elements/CaseQuantity.html>.
# fileName
phdd:fileName a rdf:Property, owl:DatatypeProperty;
    rdfs:label "File name"@en;rdfs:comment "The file name or URI of the table.	Equivalent element in DDI 3.2: pi:DataFileIdentificationDDI 3.2 Documentation: http://www.ddialliance.org/Specification/DDI-Lifecycle/3.2/XMLSchema/FieldLevelDocumentation/schemas/physicalinstance_xsd/elements/DataFileIdentification.html"@en;
    rdfs:domain phdd:TableDescription;
    rdfs:range [a owl:Class; owl:unionOf (phdd:TableDescription phdd:InputProgram)];
    rdfs:isDefinedBy <http://rdf-vocabulary.ddialliance.org/phdd>.
# recordsPerCase
phdd:recordsPerCase a rdf:Property, owl:DatatypeProperty;
    rdfs:label "Records per case"@en;rdfs:comment "The number of records per case. Multiple records could represent one case. The default is 1."@en;
    rdfs:domain phdd:TableDescription;
    rdfs:range xsd:positiveInteger;
    rdfs:isDefinedBy <http://rdf-vocabulary.ddialliance.org/phdd>.
# overallRecordCount
phdd:overallRecordCount a rdf:Property, owl:DatatypeProperty;
    rdfs:label "Overall record count"@en;rdfs:comment "Overall record count in the table.Equivalent element in DDI 3.2: pi:OverallRecordCountDDI 3.2 Documentation: http://www.ddialliance.org/Specification/DDI-Lifecycle/3.2/XMLSchema/FieldLevelDocumentation/schemas/physicalinstance_xsd/elements/OverallRecordCount.html"@en;
    rdfs:domain phdd:TableDescription;
    rdfs:range xsd:nonNegativeInteger;
    rdfs:isDefinedBy <http://rdf-vocabulary.ddialliance.org/phdd>;
    rdfs:isDefinedBy <http://www.ddialliance.org/Specification/DDI-Lifecycle/3.2/XMLSchema/FieldLevelDocumentation/schemas/physicalinstance_xsd/elements/OverallRecordCount.html>.
# recordLength
phdd:recordLength a rdf:Property, owl:DatatypeProperty;
    rdfs:label "Record length"@en;rdfs:comment "The length of a record with fixed length."@en;
    rdfs:domain phdd:FixedRecordLength;
    rdfs:range xsd:positiveInteger;
    rdfs:isDefinedBy <http://rdf-vocabulary.ddialliance.org/phdd>.
# delimiter
phdd:delimiter a rdf:Property, owl:DatatypeProperty;
    rdfs:label "Delimiter"@en;rdfs:comment "Defines the delimiter used to separate variables in a delimited record.Equivalent element in DDI 3.2: p:DelimiterDDI 3.2 Documentation: http://www.ddialliance.org/Specification/DDI-Lifecycle/3.2/XMLSchema/FieldLevelDocumentation/schemas/physicaldataproduct_xsd/elements/Delimiter.html"@en;
    rdfs:domain phdd:Delimited;
    rdfs:range xsd:string;
    rdfs:isDefinedBy <http://rdf-vocabulary.ddialliance.org/phdd>;
    rdfs:isDefinedBy <http://www.ddialliance.org/Specification/DDI-Lifecycle/3.2/XMLSchema/FieldLevelDocumentation/schemas/physicaldataproduct_xsd/elements/Delimiter.html>.
# textQualifier
phdd:textQualifier a rdf:Property, owl:DatatypeProperty;
    rdfs:label "text qualifier"@en;rdfs:comment "Use for delimited files to designate the which text qualifier, if any, was used. Valid values include: single quote, double quote, and none.Equivalent element in DDI 3.2: p:RecordLayout/@textQualifierDDI 3.2 Documentation: http://www.ddialliance.org/Specification/DDI-Lifecycle/3.2/XMLSchema/FieldLevelDocumentation/schemas/physicaldataproduct_xsd/complexTypes/BaseRecordLayoutType.html#a5"@en;
    rdfs:domain phdd:Delimited;
    rdfs:range xsd:string;
    rdfs:isDefinedBy <http://rdf-vocabulary.ddialliance.org/phdd>;
    rdfs:isDefinedBy <http://www.ddialliance.org/Specification/DDI-Lifecycle/3.2/XMLSchema/FieldLevelDocumentation/schemas/physicaldataproduct_xsd/complexTypes/BaseRecordLayoutType.html#a5>.
# consecutiveDelimitersAsOne
phdd:consecutiveDelimitersAsOne a rdf:Property, owl:DatatypeProperty;
    rdfs:label "consecutive delimiters as one"@en;rdfs:comment "Indicates how consecutive delimiters should be handed by the software.Equivalent element in DDI 3.2: p:Delimiter/@treatConsecutiveDelimiterAsOneDDI 3.2 Documentation: http://www.ddialliance.org/Specification/DDI-Lifecycle/3.2/XMLSchema/FieldLevelDocumentation/schemas/reusable_xsd/complexTypes/DelimiterType.html#a6"@en;
    rdfs:domain phdd:Delimited;
    rdfs:range xsd:boolean;
    rdfs:isDefinedBy <http://rdf-vocabulary.ddialliance.org/phdd>;
    rdfs:isDefinedBy <http://www.ddialliance.org/Specification/DDI-Lifecycle/3.2/XMLSchema/FieldLevelDocumentation/schemas/reusable_xsd/complexTypes/DelimiterType.html#a6>.
# namesOnFirstRow
phdd:namesOnFirstRow a rdf:Property, owl:DatatypeProperty;
    rdfs:label "Names on first row"@en;rdfs:comment "Indicates if the first row of the table contains the names of the columns. Default is true.Equivalent element in DDI 3.2: p:RecordLayout/@namesOnFirstRowDDI 3.2 Documentation: http://www.ddialliance.org/Specification/DDI-Lifecycle/3.2/XMLSchema/FieldLevelDocumentation/schemas/physicaldataproduct_xsd/complexTypes/RecordLayoutType.html#a5"@en;
    rdfs:domain phdd:Delimited;
    rdfs:range xsd:boolean;
    rdfs:isDefinedBy <http://rdf-vocabulary.ddialliance.org/phdd>;
    rdfs:isDefinedBy <http://www.ddialliance.org/Specification/DDI-Lifecycle/3.2/XMLSchema/FieldLevelDocumentation/schemas/physicaldataproduct_xsd/complexTypes/RecordLayoutType.html#a5>.
# firstDataLine
phdd:firstDataLine a rdf:Property, owl:DatatypeProperty;
    rdfs:label "First data line"@en;rdfs:comment "First line where the data start. Default is 2."@en;
    rdfs:domain phdd:Delimited;
    rdfs:range xsd:positiveInteger;
    rdfs:isDefinedBy <http://rdf-vocabulary.ddialliance.org/phdd>.
# defaultDecimalSeparator
phdd:defaultDecimalSeparator a rdf:Property, owl:DatatypeProperty;
    rdfs:label "Default decimal separator"@en;rdfs:comment "The character used to separate whole numbers from decimals expressed as a one character string.Equivalent element in DDI 3.2: r:DefaultDecimalSeparatorDDI 3.2 Documentation: http://www.ddialliance.org/Specification/DDI-Lifecycle/3.2/XMLSchema/FieldLevelDocumentation/schemas/reusable_xsd/elements/DefaultDecimalSeparator.html"@en;
    rdfs:domain phdd:TableStructure;
    rdfs:range xsd:string;
    rdfs:isDefinedBy <http://www.ddialliance.org/Specification/DDI-Lifecycle/3.2/XMLSchema/FieldLevelDocumentation/schemas/reusable_xsd/elements/DefaultDecimalSeparator.html>;
    rdfs:isDefinedBy <http://rdf-vocabulary.ddialliance.org/phdd>.
# defaultDigitGroupSeparator
phdd:defaultDigitGroupSeparator a rdf:Property, owl:DatatypeProperty;
    rdfs:label "default digit group separator"@en;rdfs:comment "The character used to separate the component of whole numbers (thousands, millions, etc.) expressed as a one character string.Equivalent element in DDI 3.2: r:DefaultDigitGroupSeparatorDDI 3.2 Documentation: http://www.ddialliance.org/Specification/DDI-Lifecycle/3.2/XMLSchema/FieldLevelDocumentation/schemas/reusable_xsd/elements/DefaultDigitGroupSeparator.html"@en;
    rdfs:domain phdd:TableStructure;
    rdfs:range xsd:string;
    rdfs:isDefinedBy <http://rdf-vocabulary.ddialliance.org/phdd>;
    rdfs:isDefinedBy <http://www.ddialliance.org/Specification/DDI-Lifecycle/3.2/XMLSchema/FieldLevelDocumentation/schemas/reusable_xsd/elements/DefaultDigitGroupSeparator.html>.
# defaultDecimalPositions
phdd:defaultDecimalPositions a rdf:Property, owl:DatatypeProperty;
    rdfs:label "Default decimal positions"@en;rdfs:comment "Number of decimal places for data values with an implied decimal separator. It applies to the whole table. Another expression is decimal scaling factor. Default is 0.Equivalent element in DDI 3.2: r:DefaultDecimalPositionsDDI 3.2 Documentation: http://www.ddialliance.org/Specification/DDI-Lifecycle/3.2/XMLSchema/FieldLevelDocumentation/schemas/reusable_xsd/elements/DefaultDecimalPositions.html"@en;
    rdfs:domain phdd:TableStructure;
    rdfs:range xsd:positiveInteger;
    rdfs:isDefinedBy <http://rdf-vocabulary.ddialliance.org/phdd>;
    rdfs:isDefinedBy <http://www.ddialliance.org/Specification/DDI-Lifecycle/3.2/XMLSchema/FieldLevelDocumentation/schemas/reusable_xsd/elements/DefaultDecimalPositions.html>.
# newLine
phdd:newLine a rdf:Property, owl:DatatypeProperty;
    rdfs:label "New line"@en;rdfs:comment "Specifies the end-of-line (EOL) marker used in the file as produced. If no value is provided assume the use of a CRLF (carriage return and line feed)Equivalent element in DDI 3.2: p:EndOfLineMarkerDDI 3.2 Documentation: http://www.ddialliance.org/Specification/DDI-Lifecycle/3.2/XMLSchema/FieldLevelDocumentation/schemas/physicaldataproduct_xsd/elements/EndOfLineMarker.html"@en;
    rdfs:domain phdd:TableStructure;
    rdfs:range xsd:string;
    rdfs:isDefinedBy <http://rdf-vocabulary.ddialliance.org/phdd>;
    rdfs:isDefinedBy <http://www.ddialliance.org/Specification/DDI-Lifecycle/3.2/XMLSchema/FieldLevelDocumentation/schemas/physicaldataproduct_xsd/elements/EndOfLineMarker.html>.
# columnPosition
phdd:columnPosition a rdf:Property, owl:DatatypeProperty;
    rdfs:label "Column position"@en;rdfs:comment "Position number of the column for delimited records.Equivalent element in DDI 3.2: ArrayPositionDDI 3.2 Documentation: http://www.ddialliance.org/Specification/DDI-Lifecycle/3.2/XMLSchema/FieldLevelDocumentation/schemas/physicaldataproduct_xsd/elements/ArrayPosition.html"@en;
    rdfs:domain phdd:DelimitedColumnDescription;
    rdfs:range xsd:positiveInteger;
    rdfs:isDefinedBy <http://rdf-vocabulary.ddialliance.org/phdd>;
    rdfs:isDefinedBy <http://www.ddialliance.org/Specification/DDI-Lifecycle/3.2/XMLSchema/FieldLevelDocumentation/schemas/physicaldataproduct_xsd/elements/ArrayPosition.html>.
# recommendedDataType
phdd:recommendedDataType a rdf:Property, owl:DatatypeProperty;
    rdfs:label "Recommended data type"@en;rdfs:comment "The data type as recommended by the data producer.Equivalent element in DDI 3.2: r:RecommendedDataTypeDDI 3.2 Documentation: http://www.ddialliance.org/Specification/DDI-Lifecycle/3.2/XMLSchema/FieldLevelDocumentation/schemas/reusable_xsd/elements/RecommendedDataType.html"@en;
    rdfs:domain phdd:ColumnDescription;
    rdfs:range xsd:string;
    rdfs:isDefinedBy <http://rdf-vocabulary.ddialliance.org/phdd>;
    rdfs:isDefinedBy <http://www.ddialliance.org/Specification/DDI-Lifecycle/3.2/XMLSchema/FieldLevelDocumentation/schemas/reusable_xsd/elements/RecommendedDataType.html>.

# decimalPositions
phdd:decimalPositions a rdf:Property, owl:DatatypeProperty;
    rdfs:label "Decimal positions"@en;rdfs:comment "Number of decimal places for data values with an implied decimal separator. Another expression is decimal scaling factor. Default is 0.Equivalent element in DDI 3.2: p:DecimalPositionsDDI 3.2 Documentation: http://www.ddialliance.org/Specification/DDI-Lifecycle/3.2/XMLSchema/FieldLevelDocumentation/schemas/physicaldataproduct_xsd/elements/DecimalPositions.html"@en;
    rdfs:domain phdd:ColumnDescription;
    rdfs:range xsd:positiveInteger;
    rdfs:isDefinedBy <http://rdf-vocabulary.ddialliance.org/phdd>;
    rdfs:isDefinedBy <http://www.ddialliance.org/Specification/DDI-Lifecycle/3.2/XMLSchema/FieldLevelDocumentation/schemas/physicaldataproduct_xsd/elements/DecimalPositions.html>.
# recordNumber
phdd:recordNumber a rdf:Property, owl:DatatypeProperty;
    rdfs:label "Record number"@en;rdfs:comment "The record number where this data item ('Column') is included. This applies only to tables with cases using multiple records. Default is 1.Related element in DDI 3.2: p:PhysicalRecordSegment/@segmentOrderDDI 3.2 Documentation: http://www.ddialliance.org/Specification/DDI-Lifecycle/3.2/XMLSchema/FieldLevelDocumentation/schemas/physicaldataproduct_xsd/complexTypes/PhysicalRecordSegmentType.html#a6"@en;
    rdfs:domain phdd:ColumnDescription;
    rdfs:range xsd:positiveInteger;
    rdfs:isDefinedBy <http://rdf-vocabulary.ddialliance.org/phdd>;
    rdfs:isDefinedBy <http://www.ddialliance.org/Specification/DDI-Lifecycle/3.2/XMLSchema/FieldLevelDocumentation/schemas/physicaldataproduct_xsd/complexTypes/PhysicalRecordSegmentType.html#a6>.
# startPosition
phdd:startPosition a rdf:Property, owl:DatatypeProperty;
    rdfs:label "start position"@en;rdfs:comment "start position"@en;
    rdfs:domain phdd:FixedColumnDescription;
    rdfs:label "Start position"@en;rdfs:comment "Position of the first character of the column in a table with fixed record length.Equivalent element in DDI 3.2: p:StartPositionDDI 3.2 Documentation: http://www.ddialliance.org/Specification/DDI-Lifecycle/3.2/XMLSchema/FieldLevelDocumentation/schemas/physicaldataproduct_xsd/elements/StartPosition.html"@en;
    rdfs:range xsd:positiveInteger;
    rdfs:isDefinedBy <http://rdf-vocabulary.ddialliance.org/phdd>;
    rdfs:isDefinedBy <http://www.ddialliance.org/Specification/DDI-Lifecycle/3.2/XMLSchema/FieldLevelDocumentation/schemas/physicaldataproduct_xsd/elements/StartPosition.html>.
# endPosition
phdd:endPosition a rdf:Property, owl:DatatypeProperty;
    rdfs:label "end position"@en;rdfs:comment "end position"@en;
    rdfs:domain phdd:FixedColumnDescription;
    rdfs:label "End position"@en;rdfs:comment "Position of the last character of the column in a table with fixed record length. Must be specified if a value for 'width' is not provided.Equivalent element in DDI 3.2: p:EndPositionDDI 3.2 Documentation: http://www.ddialliance.org/Specification/DDI-Lifecycle/3.2/XMLSchema/FieldLevelDocumentation/schemas/physicaldataproduct_xsd/elements/EndPosition.html"@en;
    rdfs:range xsd:positiveInteger;
    rdfs:isDefinedBy <http://rdf-vocabulary.ddialliance.org/phdd>;
    rdfs:isDefinedBy <http://www.ddialliance.org/Specification/DDI-Lifecycle/3.2/XMLSchema/FieldLevelDocumentation/schemas/physicaldataproduct_xsd/elements/EndPosition.html>.
# width
phdd:width a rdf:Property, owl:DatatypeProperty;
    rdfs:label "width"@en;rdfs:comment "width"@en;
    rdfs:domain phdd:FixedColumnDescription;rdfs:comment "Column width in a table with fixed record length. Must be specified if a value for 'endPosition' is not provided.Equivalent element in DDI 3.2: p:WidthDDI 3.2 Documentation: http://www.ddialliance.org/Specification/DDI-Lifecycle/3.2/XMLSchema/FieldLevelDocumentation/schemas/physicaldataproduct_xsd/elements/Width.html"@en;
    rdfs:range xsd:positiveInteger;
    rdfs:isDefinedBy <http://rdf-vocabulary.ddialliance.org/phdd>;
    rdfs:isDefinedBy <http://www.ddialliance.org/Specification/DDI-Lifecycle/3.2/XMLSchema/FieldLevelDocumentation/schemas/physicaldataproduct_xsd/elements/Width.html>.

#################################################################
# Object properties
#################################################################

# inputProgram
phdd:inputProgram a rdf:Property, owl:ObjectProperty;
    rdfs:label "Input program"@en;rdfs:comment "Program or program statements for reading the data.Related element in DDI 3.2: r:CommandFileDDI 3.2 Documentation: http://www.ddialliance.org/Specification/DDI-Lifecycle/3.2/XMLSchema/FieldLevelDocumentation/schemas/reusable_xsd/elements/CommandFile.html"@en;
    rdfs:domain phdd:TableDescription;
    rdfs:range phdd:InputProgram;
    rdfs:isDefinedBy <http://rdf-vocabulary.ddialliance.org/phdd>.

# isDescribedBy
phdd:isDescribedBy a rdf:Property, owl:ObjectProperty;
    rdfs:label "is described by"@en;rdfs:comment "is described by"@en;
    rdfs:domain [a owl:Class; owl:unionOf (phdd:Table phdd:Column)];
    rdfs:range [a owl:Class; owl:unionOf (phdd:TableDescription phdd:ColumnDescription)];
    rdfs:isDefinedBy <http://rdf-vocabulary.ddialliance.org/phdd>.
# isStructuredBy
phdd:isStructuredBy a rdf:Property, owl:ObjectProperty;
    rdfs:label "is structured by"@en;rdfs:comment "is structured by"@en;
    rdfs:domain phdd:Table;
    rdfs:range phdd:TableStructure;
    rdfs:isDefinedBy <http://rdf-vocabulary.ddialliance.org/phdd>.
# column
phdd:column a rdf:Property, owl:ObjectProperty;
    rdfs:label "column"@en;rdfs:comment "A column of a table. Other terms are variable or data item.Equivalent class in Disco: VariableDisco documentation: http://rdf-vocabulary.ddialliance.org/discovery.html#variable-and-variable-definitionEquivalent element in DDI 3.2: l:VariableDDI 3.2 Documentation:  http://www.ddialliance.org/Specification/DDI-Lifecycle/3.2/XMLSchema/FieldLevelDocumentation/schemas/logicalproduct_xsd/elements/Variable.html"@en;
    rdfs:domain phdd:TableStructure;
    rdfs:range phdd:Column;
    rdfs:isDefinedBy <http://rdf-vocabulary.ddialliance.org/phdd>.
# defaultLocale
phdd:defaultLocale a rdf:Property, owl:ObjectProperty;
    rdfs:label "Default locale"@en;rdfs:comment "The default locale of text in the table. It is a set of parameters that defines the country, and any special variant preferences similar to BCP 47. The language can be defined by 'defaultLanguage'. Supports the use of an external controlled vocabulary in SKOS.Related element in DDI 3.2: p:LocaleOfDataDDI 3.2 Documentation: http://www.ddialliance.org/Specification/DDI-Lifecycle/3.2/XMLSchema/FieldLevelDocumentation/schemas/physicaldataproduct_xsd/elements/LocaleOfData.html"@en;
    rdfs:domain phdd:TableStructure;
    rdfs:range [a owl:Class; owl:unionOf (skos:Concept xsd:string)];
    rdfs:isDefinedBy <http://rdf-vocabulary.ddialliance.org/phdd>;
    rdfs:seeAlso <http://www.ddialliance.org/Specification/DDI-Lifecycle/3.2/XMLSchema/FieldLevelDocumentation/schemas/physicaldataproduct_xsd/elements/LocaleOfData.html>.
# characterSet
phdd:characterSet a rdf:Property, owl:ObjectProperty;
    rdfs:label "character set"@en;rdfs:comment "The character set or encoding used in the table. Supports the use of an external controlled vocabulary in SKOS.Equivalent element in DDI 3.2: CharacterSetDDI 3.2 Documentation: http://www.ddialliance.org/Specification/DDI-Lifecycle/3.2/XMLSchema/FieldLevelDocumentation/schemas/reusable_xsd/elements/CharacterSet.html"@en;
    rdfs:domain phdd:TableStructure;
    rdfs:range [a owl:Class; owl:unionOf (skos:Concept xsd:string)];
    rdfs:isDefinedBy <http://rdf-vocabulary.ddialliance.org/phdd>;
    rdfs:isDefinedBy <http://www.ddialliance.org/Specification/DDI-Lifecycle/3.2/XMLSchema/FieldLevelDocumentation/schemas/reusable_xsd/elements/CharacterSet.html>.
# defaultLanguage
phdd:defaultLanguage a rdf:Property, owl:ObjectProperty;
    rdfs:label "Default language"@en;rdfs:comment "Default language of text in the table. Supports the use of an external controlled vocabulary in SKOS.Related element in DDI 3.2: p:LanguageOfDataDDI 3.2 Documentation: http://www.ddialliance.org/Specification/DDI-Lifecycle/3.2/XMLSchema/FieldLevelDocumentation/schemas/physicaldataproduct_xsd/elements/LanguageOfData.html"@en;
    rdfs:domain phdd:TableStructure;
    rdfs:range [a owl:Class; owl:unionOf (skos:Concept xsd:string)];
    rdfs:isDefinedBy <http://rdf-vocabulary.ddialliance.org/phdd>;
    rdfs:seeAlso <http://www.ddialliance.org/Specification/DDI-Lifecycle/3.2/XMLSchema/FieldLevelDocumentation/schemas/physicaldataproduct_xsd/elements/LanguageOfData.html>.
# storageFormat
phdd:storageFormat a rdf:Property, owl:ObjectProperty;
    rdfs:label "Storage format"@en;rdfs:comment "Definition of the storage format of data values of a column. Supports the use of an external controlled vocabulary in SKOS.Equivalent element in DDI 3.2: p:StorageFormatDDI 3.2 Documentation: http://www.ddialliance.org/Specification/DDI-Lifecycle/3.2/XMLSchema/FieldLevelDocumentation/schemas/physicaldataproduct_xsd/elements/StorageFormat.html"@en;
    rdfs:domain phdd:ColumnDescription;
    rdfs:range [a owl:Class; owl:unionOf (skos:Concept xsd:string)];
    rdfs:isDefinedBy <http://rdf-vocabulary.ddialliance.org/phdd>;
    rdfs:isDefinedBy <http://www.ddialliance.org/Specification/DDI-Lifecycle/3.2/XMLSchema/FieldLevelDocumentation/schemas/physicaldataproduct_xsd/elements/StorageFormat.html>.
# recommendedDisplayDataFormat
phdd:recommendedDisplayDataFormat a rdf:Property, owl:ObjectProperty;
    rdfs:label "Recommended display data format"@en;rdfs:comment "The recommended display format of the data values of a column. Supports the use of an external controlled vocabulary in SKOS.Equivalent element in DDI 3.2: r:GenericOutputFormatDDI 3.2 Documentation: http://www.ddialliance.org/Specification/DDI-Lifecycle/3.2/XMLSchema/FieldLevelDocumentation/schemas/reusable_xsd/elements/GenericOutputFormat.html"@en;
    rdfs:domain phdd:ColumnDescription;
    rdfs:range [a owl:Class; owl:unionOf (skos:Concept xsd:string)];
    rdfs:isDefinedBy <http://rdf-vocabulary.ddialliance.org/phdd>;rdfs:isDefinedBy <http://www.ddialliance.org/Specification/DDI-Lifecycle/3.2/XMLSchema/FieldLevelDocumentation/schemas/reusable_xsd/elements/GenericOutputFormat.html>.
